create simulate layer for blob_hash and origin, with corresponding link layer

RocqOfRust/revm/revm_interpreter/instructions/links/tx_info.v
@@ -1,5 +1,8 @@
 Require Import links.RocqOfRust.
+Require Import alloy_primitives.bits.links.address.
 Require Import alloy_primitives.bits.links.fixed.
+Require Import alloy_primitives.links.aliases.
+Require Import core.links.default.
 Require Import core.convert.links.mod.
 Require Import core.convert.links.num.
 Require Import core.links.cmp.
@@ -18,6 +21,37 @@ Require Import revm.revm_interpreter.links.interpreter.
 Require Import revm.revm_interpreter.links.interpreter_types.
 Require Import revm.revm_primitives.links.hardfork.
 Require Import ruint.links.from.
+Require Import ruint.links.lib.
+
+Module Impl_Default_for_U256.
+  Definition Self : Set := aliases.U256.t.
+
+  Instance run_default :
+    Run.Trait
+      (ruint.lib.Impl_core_default_Default_for_ruint_Uint_BITS_LIMBS.default
+        (Value.Integer IntegerKind.Usize 256)
+        (Value.Integer IntegerKind.Usize 4))
+      [] [] []
+      Self.
+  Proof.
+    constructor.
+    run_symbolic.
+  Defined.
+
+  Instance method_default : Default.Method_default Self.
+  Proof.
+    eexists.
+    { constructor.
+      eapply IsTraitMethod.Defined.
+      { apply ruint.lib.Impl_core_default_Default_for_ruint_Uint_BITS_LIMBS.Implements. }
+      { reflexivity. }
+    }
+    { typeclasses eauto. }
+  Defined.
+
+  Instance run : Default.Run Self := {}.
+End Impl_Default_for_U256.
+Export (hints) Impl_Default_for_U256.
 
 (*
 pub fn gasprice<WIRE: InterpreterTypes, H: Host + ?Sized>(
@@ -57,8 +91,7 @@ Global Opaque run_gasprice.
 
 (*
 pub fn origin<WIRE: InterpreterTypes, H: Host + ?Sized>(
-    interpreter: &mut Interpreter<WIRE>,
-    host: &mut H,
+    context: InstructionContext<'_, H, WIRE>,
 )
 *)
 Instance run_origin
@@ -67,28 +100,34 @@ Instance run_origin
   (run_InterpreterTypes_for_WIRE : InterpreterTypes.Run WIRE WIRE_types)
   {H_types : Host.Types.t} `{Host.Types.AreLinks H_types}
   (run_Host_for_H : Host.Run H H_types)
-  (interpreter : '&mut (Interpreter.t WIRE WIRE_types))
-  (host : '&mut H) :
+  (context : InstructionContext.t H WIRE WIRE_types) :
   Run.Trait
-    instructions.tx_info.origin [] [ Φ WIRE; Φ H ] [ φ interpreter; φ host ]
+    instructions.tx_info.origin [] [ Φ WIRE; Φ H ] [ φ context ]
     unit.
 Proof.
   constructor.
-  destruct run_InterpreterTypes_for_WIRE.
+  destruct run_InterpreterTypes_for_WIRE eqn:?.
   destruct run_StackTrait_for_Stack.
   destruct run_LoopControl_for_Control.
   destruct run_Host_for_H.
+  destruct run_BlockGetter_for_Self.
+  destruct run_Block_for_Block.
   destruct run_TransactionGetter_for_Self.
-  destruct (Impl_Into_for_From_T.run Impl_From_FixedBytes_32_for_U256.run).
+  destruct run_Transaction_for_Transaction.
   run_symbolic.
-  (* dyn type *)
-Admitted.
+  { eapply (@Host.run_caller
+      ('&mut H)
+      _
+      (@Impl_Host_for_RefMut.method_caller H _ method_caller)
+      (Ref.cast_to Pointer.Kind.Ref sub_ref1)). }
+  Unshelve.
+  all: eapply Impl_Address.run_into_word.
+Defined.
 Global Opaque run_origin.
 
 (*
 pub fn blob_hash<WIRE: InterpreterTypes, H: Host + ?Sized>(
-    interpreter: &mut Interpreter<WIRE>,
-    host: &mut H,
+    context: InstructionContext<'_, H, WIRE>,
 )
 *)
 Instance run_blob_hash
@@ -97,40 +136,30 @@ Instance run_blob_hash
   (run_InterpreterTypes_for_WIRE : InterpreterTypes.Run WIRE WIRE_types)
   {H_types : Host.Types.t} `{Host.Types.AreLinks H_types}
   (run_Host_for_H : Host.Run H H_types)
-  (interpreter : '&mut (Interpreter.t WIRE WIRE_types))
-  (host : '&mut H) :
+  (context : InstructionContext.t H WIRE WIRE_types) :
   Run.Trait
-    instructions.tx_info.blob_hash [] [ Φ WIRE; Φ H ] [ φ interpreter; φ host ]
+    instructions.tx_info.blob_hash [] [ Φ WIRE; Φ H ] [ φ context ]
     unit.
 Proof.
   constructor.
-  destruct run_InterpreterTypes_for_WIRE.
+  destruct run_InterpreterTypes_for_WIRE eqn:?.
+  destruct run_RuntimeFlag_for_RuntimeFlag.
   destruct run_StackTrait_for_Stack.
   destruct run_LoopControl_for_Control.
-  destruct run_RuntimeFlag_for_RuntimeFlag.
   destruct run_Host_for_H.
+  destruct run_BlockGetter_for_Self.
+  destruct run_Block_for_Block.
   destruct run_TransactionGetter_for_Self.
-  destruct Impl_TryFrom_u64_for_usize.run.
-  destruct Impl_PartialEq_for_TransactionType.run.
-  destruct (Impl_Transaction_for_Ref_Transaction.run _ _ run_Transaction_for_Transaction).
   destruct run_Transaction_for_Transaction.
-  destruct run_Into_for_TransactionType.
-  destruct run_Eip4844Tx_for_Eip4844.
+  destruct Impl_TryFrom_u64_for_usize.run.
   run_symbolic.
-  (* repeat (
-        erewrite IsTraitAssociatedType_eq ||
-        match goal with
-        | H : _ |- _ => exact H
-        end
-      ).
-      2: { admit. }
-  run_symbolic.
-  2: {
-    generalize tx; clear; intros []; cbn in *.
-  }
-      2: {
-
-        generalize Transaction_IsAssociated; clear; intros.
-      } *)
-Admitted.
+  { eapply (@Host.run_blob_hash
+      ('&mut H)
+      _
+      (@Impl_Host_for_RefMut.method_blob_hash H _ method_blob_hash)). }
+  Unshelve.
+  all: eapply Impl_Option.run_unwrap_or_default.
+  Unshelve.
+  all: typeclasses eauto.
+Defined.
 Global Opaque run_blob_hash.
