RocqOfRust/revm/revm_interpreter/instructions/simulate/tx_info/blob_hash.v
@@ -1,0 +1,143 @@
+Require Import simulate.RocqOfRust.
+Require Import alloy_primitives.links.aliases.
+Require Import core.simulate.default.
+Require Import core.simulate.option.
+Require Import revm.revm_context_interface.links.host.
+Require Import revm.revm_context_interface.simulate.host.
+Require Import revm.revm_interpreter.instructions.links.tx_info.
+Require Import revm.revm_interpreter.instructions.simulate.macros.
+Require Import revm.revm_interpreter.links.instruction_context.
+Require Import revm.revm_interpreter.links.interpreter.
+Require Import revm.revm_interpreter.links.interpreter_types.
+Require Import revm.revm_interpreter.simulate.interpreter_types.
+Require Import revm.revm_primitives.links.hardfork.
+Require Import revm.revm_primitives.simulate.hardfork.
+Require Import ruint.simulate.lib.
+
+Module Sim_Default_for_U256.
+  Instance I : Default.C aliases.U256.t := {|
+    Default.default := Impl_Uint.ZERO;
+  |}.
+
+  Module Eq.
+    Instance I :
+      @Default.Eq.C
+        aliases.U256.t
+        _
+        Impl_Default_for_U256.run
+        Sim_Default_for_U256.I.
+    Proof.
+      constructor; intros.
+      s. {
+        apply Impl_Uint.ZERO_eq.
+      }
+      s.
+    Qed.
+  End Eq.
+  Export (hints) Eq.
+End Sim_Default_for_U256.
+Export (hints) Sim_Default_for_U256.
+
+Definition blob_hash
+    {WIRE H : Set} `{Link WIRE} `{Link H}
+    {WIRE_types : InterpreterTypes.Types.t} `{InterpreterTypes.Types.AreLinks WIRE_types}
+    {IInterpreterTypes : InterpreterTypes.C WIRE_types}
+    {H_types : Host.Types.t} `{Host.Types.AreLinks H_types}
+    {IHost : Host.C H H_types}
+    (interpreter : Interpreter.t WIRE WIRE_types)
+    (host : H) :
+    Interpreter.t WIRE WIRE_types * H :=
+  check_macro interpreter SpecId.CANCUN (fun interpreter => (interpreter, host)) (fun interpreter =>
+  popn_top_macro interpreter 0
+    (fun interpreter => (interpreter, host)) (fun _ index_stub interpreter =>
+  let index := index_stub.(RefStub.projection) interpreter.(Interpreter.stack) in
+  let index_usize := as_usize_saturated_macro index in
+  let '(hash_opt, host) := IHost.(Host.blob_hash) host index_usize in
+  let hash :=
+    match hash_opt with
+    | Some hash => hash
+    | None => Impl_Uint.ZERO
+    end in
+  let stack := index_stub.(RefStub.injection) interpreter.(Interpreter.stack) hash in
+  (interpreter <| Interpreter.stack := stack |>, host))).
+
+Lemma blob_hash_eq
+    {WIRE H : Set} `{Link WIRE} `{Link H}
+    {WIRE_types : InterpreterTypes.Types.t} `{InterpreterTypes.Types.AreLinks WIRE_types}
+    (run_InterpreterTypes_for_WIRE : InterpreterTypes.Run WIRE WIRE_types)
+    {H_types : Host.Types.t} `{Host.Types.AreLinks H_types}
+    (run_Host_for_H : Host.Run H H_types)
+    `{IInterpreterTypes : !InterpreterTypes.C WIRE_types}
+    `{InterpreterTypesEq :
+      !InterpreterTypes.Eq.t WIRE WIRE_types run_InterpreterTypes_for_WIRE IInterpreterTypes}
+    `{IHost : !Host.C H H_types}
+    `{HostEq : !Host.Eq.t IHost}
+    (interpreter : Interpreter.t WIRE WIRE_types)
+    (host : H) :
+  let ref_interpreter := make_ref 0 in
+  let ref_host := make_ref (A := H) 1 in
+  let context := {|
+    instruction_context.InstructionContext.interpreter := ref_interpreter;
+    instruction_context.InstructionContext.host := ref_host;
+  |} in
+  let result := blob_hash interpreter host in
+  {{
+    SimulateM.eval_f
+      (run_blob_hash run_InterpreterTypes_for_WIRE run_Host_for_H context)
+      [interpreter; host]%stack 🌲
+    (
+      Output.Success tt,
+      [fst result; snd result]%stack
+    )
+  }}.
+Proof.
+  intros.
+  subst result.
+  with_strategy transparent [run_blob_hash] unfold blob_hash, run_blob_hash; cbn.
+  check_macro_eq InterpreterTypesEq.
+  popn_top_macro_eq InterpreterTypesEq.
+  eapply Run.Call; [
+    eapply Impl_Option.unwrap_unchecked_eq;
+    reflexivity
+  |].
+  cbn.
+  match goal with
+  | top : RefStub.t _ aliases.U256.t,
+    stack_after : WIRE_types.(InterpreterTypes.Types.Stack) |- _ =>
+      eapply Run.Let with
+        (result := (
+          Output.Success
+            (as_usize_saturated_macro
+              (top.(RefStub.projection) stack_after)),
+          _
+        ))
+  end.
+  -
+    as_usize_saturated_macro_eq.
+  -
+    set (index := as_usize_saturated_macro (t0.(RefStub.projection) s)).
+    match goal with
+    | |- context [IHost.(Host.blob_hash) host index] =>
+        destruct (IHost.(Host.blob_hash) host index) as [hash_opt host_after] eqn:?
+    end.
+    s. {
+      eapply Run.Call.
+      {
+        pose proof
+          (HostEq.(Host.Eq.blob_hash)
+            (interpreter<|Interpreter.stack:= s|>)
+            host
+            index
+            ([tt; tt; index]%stack)) as H_blob_hash.
+        cbn [SimulateM.eval_f] in H_blob_hash.
+        exact H_blob_hash.
+      }
+      s.
+    }
+    rewrite Heqp; cbn.
+    s. {
+      eapply Impl_Option.unwrap_or_default_eq.
+    }
+    cbn.
+    destruct hash_opt; s.
+Qed.
